Tap

Gt3/Cotree/Basic.lean
@@ -5,406 +5,408 @@ namespace Gt3
 
 open NumChildren BinderList HasChildren FlatChildren
 
-inductive Node.SimRelUpto
-  (stop : Prop) {α β} [BinderList α] [BinderList β] (rel : α → β → Prop) {ι₁ ι₂}
-  (lhs : ι₁ → Node α ι₁ → Prop) (rhs : ι₂ → Node β ι₂ → Prop) : ℕ → ι₁ → ι₂ → Prop
-  | done (i₁ i₂) : stop → SimRelUpto stop rel lhs rhs 0 i₁ i₂
-  | node {i₁ i₂ n₁ n₂}
-    (hn₁ : lhs i₁ n₁) (hn₂ : rhs i₂ n₂)
-    (tag : rel n₁.tag n₂.tag)
-    (numChildren : numChildren n₁.tag = numChildren n₂.tag)
-    {gas}
-    (children :
-      ∀ j, SimRelUpto stop rel lhs rhs gas
-            (getChild n₁ j) (getChild n₂ (j.cast numChildren)))
-    : SimRelUpto stop rel lhs rhs (gas + 1) i₁ i₂
+-- inductive Node.SimRelUpto
+--   (stop : Prop) {α β} [BinderList α] [BinderList β] (rel : α → β → Prop) {ι₁ ι₂}
+--   (lhs : ι₁ → Node α ι₁ → Prop) (rhs : ι₂ → Node β ι₂ → Prop) : ℕ → ι₁ → ι₂ → Prop
+--   | done (i₁ i₂) : stop → SimRelUpto stop rel lhs rhs 0 i₁ i₂
+--   | node {i₁ i₂ n₁ n₂}
+--     (hn₁ : lhs i₁ n₁) (hn₂ : rhs i₂ n₂)
+--     (tag : rel n₁.tag n₂.tag)
+--     (numChildren : numChildren n₁.tag = numChildren n₂.tag)
+--     {gas}
+--     (children :
+--       ∀ j, SimRelUpto stop rel lhs rhs gas
+--             (getChild n₁ j) (getChild n₂ (j.cast numChildren)))
+--     : SimRelUpto stop rel lhs rhs (gas + 1) i₁ i₂
 
-def Node.SimRel {α β} [BinderList α] [BinderList β] (rel : α → β → Prop) {ι₁ ι₂}
-  (lhs : ι₁ → Node α ι₁ → Prop) (rhs : ι₂ → Node β ι₂ → Prop) (i₁ : ι₁) (i₂ : ι₂) : Prop
-  := ∀n, Node.SimRelUpto ⊤ rel lhs rhs n i₁ i₂
+-- def Node.SimRel {α β} [BinderList α] [BinderList β] (rel : α → β → Prop) {ι₁ ι₂}
+--   (lhs : ι₁ → Node α ι₁ → Prop) (rhs : ι₂ → Node β ι₂ → Prop) (i₁ : ι₁) (i₂ : ι₂) : Prop
+--   := ∀n, Node.SimRelUpto ⊤ rel lhs rhs n i₁ i₂
 
-def Node.FinSimRel {α β} [BinderList α] [BinderList β] (rel : α → β → Prop) {ι₁ ι₂}
-  (lhs : ι₁ → Node α ι₁ → Prop) (rhs : ι₂ → Node β ι₂ → Prop) (i₁ : ι₁) (i₂ : ι₂) : Prop
-  := ∃ n, Node.SimRelUpto ⊥ rel lhs rhs n i₁ i₂
+-- def Node.FinSimRel {α β} [BinderList α] [BinderList β] (rel : α → β → Prop) {ι₁ ι₂}
+--   (lhs : ι₁ → Node α ι₁ → Prop) (rhs : ι₂ → Node β ι₂ → Prop) (i₁ : ι₁) (i₂ : ι₂) : Prop
+--   := ∃ n, Node.SimRelUpto ⊥ rel lhs rhs n i₁ i₂
 
-def Node.Undef
-  {α} [BinderList α] (rel : α → α → Prop) {ι}
-  (addr : ι → Node α ι → Prop) (i : ι)
-  : Prop
-  := ¬ SimRel rel addr addr i i
+-- def Node.Undef
+--   {α} [BinderList α] (rel : α → α → Prop) {ι}
+--   (addr : ι → Node α ι → Prop) (i : ι)
+--   : Prop
+--   := ¬ SimRel rel addr addr i i
 
-def Node.Undef2
-  {α} [BinderList α] (rel : α → α → Prop) {ι}
-  (lhs : ι → Node α ι → Prop) (rhs : ι → Node α ι → Prop) (i₁ : ι) (i₂ : ι)
-  : Prop
-  := Undef rel lhs i₁ ∧ Undef rel rhs i₂
+-- def Node.Undef2
+--   {α} [BinderList α] (rel : α → α → Prop) {ι}
+--   (lhs : ι → Node α ι → Prop) (rhs : ι → Node α ι → Prop) (i₁ : ι) (i₂ : ι)
+--   : Prop
+--   := Undef rel lhs i₁ ∧ Undef rel rhs i₂
 
-instance Node.Undef2.instSymm
-  {α} [BinderList α] (rel : α → α → Prop) {ι}
-  (addr : ι → Node α ι → Prop) : IsSymm ι (Node.Undef2 rel addr addr) where
-  symm _ _ h := And.intro h.right h.left
+-- instance Node.Undef2.instSymm
+--   {α} [BinderList α] (rel : α → α → Prop) {ι}
+--   (addr : ι → Node α ι → Prop) : IsSymm ι (Node.Undef2 rel addr addr) where
+--   symm _ _ h := And.intro h.right h.left
 
-instance Node.Undef2.instTrans
-  {α} [BinderList α] (rel : α → α → Prop) {ι}
-  (addr : ι → Node α ι → Prop) : IsTrans ι (Node.Undef2 rel addr addr) where
-  trans _ _ _ h1 h2 := And.intro h1.left h2.right
+-- instance Node.Undef2.instTrans
+--   {α} [BinderList α] (rel : α → α → Prop) {ι}
+--   (addr : ι → Node α ι → Prop) : IsTrans ι (Node.Undef2 rel addr addr) where
+--   trans _ _ _ h1 h2 := And.intro h1.left h2.right
 
-class Determ {β} (e : β → β → Prop) {α} (r : α → β → Prop) where
-  determ : ∀ {x y₁ y₂}, r x y₁ → r x y₂ → e y₁ y₂
+-- class Determ {β} (e : β → β → Prop) {α} (r : α → β → Prop) where
+--   determ : ∀ {x y₁ y₂}, r x y₁ → r x y₂ → e y₁ y₂
 
-theorem Determ.determ_eq {α β} {r : α → β → Prop}
-  [Determ Eq r] {x y₁ y₂} (h₁ : r x y₁) (h₂ : r x y₂) : y₁ = y₂ :=
-  determ h₁ h₂
+-- theorem Determ.determ_eq {α β} {r : α → β → Prop}
+--   [Determ Eq r] {x y₁ y₂} (h₁ : r x y₁) (h₂ : r x y₂) : y₁ = y₂ :=
+--   determ h₁ h₂
 
-class InhabAt {α} (P : α → Prop) {β} (r : α → β → Prop) where
-  rel_inhab_at : ∀ x, P x → ∃ y, r x y
+-- class InhabAt {α} (P : α → Prop) {β} (r : α → β → Prop) where
+--   rel_inhab_at : ∀ x, P x → ∃ y, r x y
 
-theorem InhabAt.rel_inhab {α β} (r : α → β → Prop)
-  [InhabAt ⊤ r] (x) : ∃ y, r x y := InhabAt.rel_inhab_at (P := ⊤) x (by simp)
+-- theorem InhabAt.rel_inhab {α β} (r : α → β → Prop)
+--   [InhabAt ⊤ r] (x) : ∃ y, r x y := InhabAt.rel_inhab_at (P := ⊤) x (by simp)
 
-open Determ InhabAt
+-- open Determ InhabAt
 
-def readMem? {α β} (mem : α → Option β) (x : α) (y : β) : Prop := mem x = y
+-- def readMem? {α β} (mem : α → Option β) (x : α) (y : β) : Prop := mem x = y
 
-instance {α β} (mem : α → Option β) : Determ Eq (readMem? mem) where
-  determ {x y₁ y₂} h₁ h₂ := by
-    simp only [readMem?] at *
-    generalize mem x = z at *
-    cases z <;> cases h₁; cases h₂; rfl
+-- instance {α β} (mem : α → Option β) : Determ Eq (readMem? mem) where
+--   determ {x y₁ y₂} h₁ h₂ := by
+--     simp only [readMem?] at *
+--     generalize mem x = z at *
+--     cases z <;> cases h₁; cases h₂; rfl
 
-def Node.SimUpto? (stop : Prop) {α β} [BinderList α] [BinderList β]
-  (rel : α → β → Prop) {ι₁ ι₂}
-  (lhs : ι₁ → Option (Node α ι₁)) (rhs : ι₂ → Option (Node β ι₂)) : ι₁ → ι₂ → ℕ → Prop
-  := fun i₁ i₂ gas => Node.SimRelUpto stop rel (readMem? lhs) (readMem? rhs) gas i₁ i₂
+-- def Node.SimUpto? (stop : Prop) {α β} [BinderList α] [BinderList β]
+--   (rel : α → β → Prop) {ι₁ ι₂}
+--   (lhs : ι₁ → Option (Node α ι₁)) (rhs : ι₂ → Option (Node β ι₂)) : ι₁ → ι₂ → ℕ → Prop
+--   := fun i₁ i₂ gas => Node.SimRelUpto stop rel (readMem? lhs) (readMem? rhs) gas i₁ i₂
 
-def Node.Sim? {α β} [BinderList α] [BinderList β]
-  (rel : α → β → Prop) {ι₁ ι₂}
-  (lhs : ι₁ → Option (Node α ι₁)) (rhs : ι₂ → Option (Node β ι₂)) (i₁ : ι₁) (i₂ : ι₂) : Prop
-  := Node.SimRel rel (readMem? lhs) (readMem? rhs) i₁ i₂
+-- def Node.Sim? {α β} [BinderList α] [BinderList β]
+--   (rel : α → β → Prop) {ι₁ ι₂}
+--   (lhs : ι₁ → Option (Node α ι₁)) (rhs : ι₂ → Option (Node β ι₂)) (i₁ : ι₁) (i₂ : ι₂) : Prop
+--   := Node.SimRel rel (readMem? lhs) (readMem? rhs) i₁ i₂
 
-def readMem {α β} (mem : α → β) (x : α) (y : β) : Prop := mem x = y
+-- def readMem {α β} (mem : α → β) (x : α) (y : β) : Prop := mem x = y
 
-def readMem.refl {α β} (mem : α → β) (x : α) : readMem mem x (mem x) := rfl
+-- def readMem.refl {α β} (mem : α → β) (x : α) : readMem mem x (mem x) := rfl
 
-instance {α β} (mem : α → β) : InhabAt ⊤ (readMem mem) where
-  rel_inhab_at x _ := ⟨mem x, rfl⟩
+-- instance {α β} (mem : α → β) : InhabAt ⊤ (readMem mem) where
+--   rel_inhab_at x _ := ⟨mem x, rfl⟩
 
-instance {α β} (mem : α → β) : Determ Eq (readMem mem) where
-  determ {x y₁ y₂} h₁ h₂ := by cases h₁; cases h₂; rfl
+-- instance {α β} (mem : α → β) : Determ Eq (readMem mem) where
+--   determ {x y₁ y₂} h₁ h₂ := by cases h₁; cases h₂; rfl
 
-def Node.SimUpto (stop : Prop) {α β} [BinderList α] [BinderList β] (rel : α → β → Prop) {ι₁ ι₂}
-  (lhs : ι₁ → Node α ι₁) (rhs : ι₂ → Node β ι₂) (gas : ℕ) : ι₁ → ι₂ → Prop
-  := Node.SimRelUpto stop rel (readMem lhs) (readMem rhs) gas
+-- def Node.SimUpto (stop : Prop) {α β} [BinderList α] [BinderList β] (rel : α → β → Prop) {ι₁ ι₂}
+--   (lhs : ι₁ → Node α ι₁) (rhs : ι₂ → Node β ι₂) (gas : ℕ) : ι₁ → ι₂ → Prop
+--   := Node.SimRelUpto stop rel (readMem lhs) (readMem rhs) gas
 
-def Node.Sim {α β} [BinderList α] [BinderList β] (rel : α → β → Prop) {ι₁ ι₂}
-  (lhs : ι₁ → Node α ι₁) (rhs : ι₂ → Node β ι₂) : ι₁ → ι₂ → Prop
-  := Node.SimRel rel (readMem lhs) (readMem rhs)
+-- def Node.Sim {α β} [BinderList α] [BinderList β] (rel : α → β → Prop) {ι₁ ι₂}
+--   (lhs : ι₁ → Node α ι₁) (rhs : ι₂ → Node β ι₂) : ι₁ → ι₂ → Prop
+--   := Node.SimRel rel (readMem lhs) (readMem rhs)
 
-def Node.FinSim {α β} [BinderList α] [BinderList β] (rel : α → β → Prop) {ι₁ ι₂}
-  (lhs : ι₁ → Node α ι₁) (rhs : ι₂ → Node β ι₂) : ι₁ → ι₂ → Prop
-  := fun i₁ i₂ => Node.FinSimRel rel (readMem lhs) (readMem rhs) i₁ i₂
+-- def Node.FinSim {α β} [BinderList α] [BinderList β] (rel : α → β → Prop) {ι₁ ι₂}
+--   (lhs : ι₁ → Node α ι₁) (rhs : ι₂ → Node β ι₂) : ι₁ → ι₂ → Prop
+--   := fun i₁ i₂ => Node.FinSimRel rel (readMem lhs) (readMem rhs) i₁ i₂
 
-section SimRel
+-- section SimRel
 
-variable {stop : Prop} {α β} [BinderList α] [BinderList β]
-        {data data₁ data₂ : α → β → Type _}
-        {rel rel₁ rel₂ : α → β → Prop}
-        {ι ι₁ ι₂}
-        {addr : ι → Node α ι → Prop} {lhs : ι₁ → Node α ι₁ → Prop} {rhs : ι₂ → Node β ι₂ → Prop}
-        {gas}
-        {i : ι} {i₁ : ι₁} {i₂ : ι₂} {n₁ n₂}
+-- variable {stop : Prop} {α β} [BinderList α] [BinderList β]
+--         {data data₁ data₂ : α → β → Type _}
+--         {rel rel₁ rel₂ : α → β → Prop}
+--         {ι ι₁ ι₂}
+--         {addr : ι → Node α ι → Prop} {lhs : ι₁ → Node α ι₁ → Prop} {rhs : ι₂ → Node β ι₂ → Prop}
+--         {gas}
+--         {i : ι} {i₁ : ι₁} {i₂ : ι₂} {n₁ n₂}
 
-namespace Node
+-- namespace Node
 
-theorem SimRelUpto.anti_gas
-  {gas₁ gas₂} (h : gas₁ ≤ gas₂) {i₁ i₂}
-  (h : SimRelUpto ⊤ rel lhs rhs gas₂ i₁ i₂) : SimRelUpto ⊤ rel lhs rhs gas₁ i₁ i₂
-  := match h, gas₁ with
-  | _, 0 => .done i₁ i₂ trivial
-  | .node hn₁ hn₂ h_tag h_numChildren h_children, gas₁ + 1 =>
-    .node hn₁ hn₂ h_tag h_numChildren
-      (fun j => anti_gas (by convert h using 0; simp) (h_children j))
+-- theorem SimRelUpto.anti_gas
+--   {gas₁ gas₂} (h : gas₁ ≤ gas₂) {i₁ i₂}
+--   (h : SimRelUpto ⊤ rel lhs rhs gas₂ i₁ i₂) : SimRelUpto ⊤ rel lhs rhs gas₁ i₁ i₂
+--   := match h, gas₁ with
+--   | _, 0 => .done i₁ i₂ trivial
+--   | .node hn₁ hn₂ h_tag h_numChildren h_children, gas₁ + 1 =>
+--     .node hn₁ hn₂ h_tag h_numChildren
+--       (fun j => anti_gas (by convert h using 0; simp) (h_children j))
 
-theorem SimRel.node
-  (hn₁ : lhs i₁ n₁) (hn₂ : rhs i₂ n₂)
-  (tag : rel n₁.tag n₂.tag)
-  (numChildren : numChildren n₁.tag = numChildren n₂.tag)
-  (children :
-    ∀ j, SimRel rel lhs rhs
-          (getChild n₁ j) (getChild n₂ (j.cast numChildren)))
-  : SimRel rel lhs rhs i₁ i₂
-  | 0 => .done i₁ i₂ trivial
-  | n + 1 => .node hn₁ hn₂ tag numChildren (fun j => children j n)
+-- theorem SimRel.node
+--   (hn₁ : lhs i₁ n₁) (hn₂ : rhs i₂ n₂)
+--   (tag : rel n₁.tag n₂.tag)
+--   (numChildren : numChildren n₁.tag = numChildren n₂.tag)
+--   (children :
+--     ∀ j, SimRel rel lhs rhs
+--           (getChild n₁ j) (getChild n₂ (j.cast numChildren)))
+--   : SimRel rel lhs rhs i₁ i₂
+--   | 0 => .done i₁ i₂ trivial
+--   | n + 1 => .node hn₁ hn₂ tag numChildren (fun j => children j n)
 
--- theorem FinSimRel.sim {i₁ i₂}
---   : FinSimRel rel lhs rhs i₁ i₂ → SimRel rel lhs rhs i₁ i₂
+-- -- theorem FinSimRel.sim {i₁ i₂}
+-- --   : FinSimRel rel lhs rhs i₁ i₂ → SimRel rel lhs rhs i₁ i₂
+-- --   | .node hn₁ hn₂ h_tag h_numChildren h_children =>
+-- --     .node hn₁ hn₂ h_tag h_numChildren (fun j => FinSimRel.sim (h_children j))
+
+-- -- theorem EFinTrace.fin_sim {i₁ i₂}
+-- --   : EFinTrace data lhs rhs i₁ i₂ → FinSimRel (fun x y => Nonempty (data x y)) lhs rhs i₁ i₂
+-- --   | .node hn₁ hn₂ h_tag h_numChildren h_children =>
+-- --     .node hn₁ hn₂ ⟨h_tag⟩ h_numChildren (fun j => fin_sim (h_children j))
+
+-- -- theorem EFinTrace.sim
+-- --   : EFinTrace data lhs rhs i₁ i₂ → SimRel (fun x y => Nonempty (data x y)) lhs rhs i₁ i₂ :=
+-- --   fun t => (t.fin_sim).sim
+
+-- theorem SimRelUpto.notBot : SimRelUpto stop ⊥ lhs rhs (gas + 1) i₁ i₂ → False
+--   | .node _ _ h_tag _ _ => by cases h_tag
+
+-- theorem SimRelUpto.ne_bot (h : SimRelUpto stop rel lhs rhs (gas + 1) i₁ i₂) : rel ≠ ⊥
+--   := fun e => (e ▸ h).notBot
+
+-- theorem SimRel.notBot (h : SimRel ⊥ lhs rhs i₁ i₂) : False := (h 1).notBot
+
+-- theorem SimRel.ne_bot (h : SimRel rel lhs rhs i₁ i₂) : rel ≠ ⊥ := (h 1).ne_bot
+
+-- theorem FinSimRel.notBot : FinSimRel ⊥ lhs rhs i₁ i₂ → False
+--   := fun ⟨gas + 1, .node _ _ h_tag _ _⟩ => by cases h_tag
+
+-- theorem FinSimRel.ne_bot (h : FinSimRel rel lhs rhs i₁ i₂) : rel ≠ ⊥
+--   := fun e => (e ▸ h).notBot
+
+-- theorem SimRelUpto.mono_rel (hrel : rel₁ ≤ rel₂) {gas} {i₁ : ι₁} {i₂ : ι₂}
+--   : SimRelUpto stop rel₁ lhs rhs gas i₁ i₂ → SimRelUpto stop rel₂ lhs rhs gas i₁ i₂
+--   | .done _ _ hs => .done i₁ i₂ hs
 --   | .node hn₁ hn₂ h_tag h_numChildren h_children =>
---     .node hn₁ hn₂ h_tag h_numChildren (fun j => FinSimRel.sim (h_children j))
+--     .node hn₁ hn₂ (hrel _ _ h_tag) h_numChildren (fun j => mono_rel hrel (h_children j))
 
--- theorem EFinTrace.fin_sim {i₁ i₂}
---   : EFinTrace data lhs rhs i₁ i₂ → FinSimRel (fun x y => Nonempty (data x y)) lhs rhs i₁ i₂
+-- theorem SimRel.mono_rel (hrel : rel₁ ≤ rel₂) {i₁ : ι₁} {i₂ : ι₂} (h : SimRel rel₁ lhs rhs i₁ i₂)
+--   : SimRel rel₂ lhs rhs i₁ i₂ := fun n => (h n).mono_rel hrel
+
+-- theorem SimRelUpto.inf [Determ Eq lhs] [Determ Eq rhs] {gas} {i₁ : ι₁} {i₂ : ι₂}
+--   : SimRelUpto stop rel₁ lhs rhs gas i₁ i₂
+--   → SimRelUpto stop rel₂ lhs rhs gas i₁ i₂
+--   → SimRelUpto stop (rel₁ ⊓ rel₂) lhs rhs gas i₁ i₂
+--   | .done _ _ hs,
+--     .done _ _ _ => .done i₁ i₂ hs
+--   | .node hn₁ hn₂ h1_tag h1_numChildren h1_children,
+--     .node hn₁' hn₂' h2_tag _ h2_children => by
+--     cases determ_eq hn₁ hn₁'
+--     cases determ_eq hn₂ hn₂'
+--     exact .node (rel := rel₁ ⊓ rel₂)
+--       hn₁ hn₂
+--       (And.intro h1_tag h2_tag) h1_numChildren
+--       (fun j => SimRelUpto.inf (h1_children j) (h2_children j))
+
+-- theorem SimRel.inf [Determ Eq lhs] [Determ Eq rhs] {i₁ : ι₁} {i₂ : ι₂}
+--   (h₁ : SimRel rel₁ lhs rhs i₁ i₂)
+--   (h₂ : SimRel rel₂ lhs rhs i₁ i₂) : SimRel (rel₁ ⊓ rel₂) lhs rhs i₁ i₂ :=
+--   fun n => SimRelUpto.inf (h₁ n) (h₂ n)
+
+-- theorem SimRelUpto.lhs_of_inf
+--   : SimRelUpto stop (rel₁ ⊓ rel₂) lhs rhs gas i₁ i₂ → SimRelUpto stop rel₁ lhs rhs gas i₁ i₂
+--   := mono_rel (by simp)
+
+-- theorem SimRelUpto.rhs_of_inf
+--   : SimRelUpto stop (rel₁ ⊓ rel₂) lhs rhs gas i₁ i₂ → SimRelUpto stop rel₂ lhs rhs gas i₁ i₂
+--   := mono_rel (by simp)
+
+-- theorem SimRelUpto.inf_iff [Determ Eq lhs] [Determ Eq rhs]
+--   : SimRelUpto stop (rel₁ ⊓ rel₂) lhs rhs gas i₁ i₂
+--     ↔ SimRelUpto stop rel₁ lhs rhs gas i₁ i₂ ∧ SimRelUpto stop rel₂ lhs rhs gas i₁ i₂ :=
+--   ⟨fun h => ⟨lhs_of_inf h, rhs_of_inf h⟩,
+--    fun ⟨h1, h2⟩ => inf h1 h2⟩
+
+-- theorem SimRel.lhs_of_inf
+--   : SimRel (rel₁ ⊓ rel₂) lhs rhs i₁ i₂ → SimRel rel₁ lhs rhs i₁ i₂ := mono_rel (by simp)
+
+-- theorem SimRel.rhs_of_inf
+--   : SimRel (rel₁ ⊓ rel₂) lhs rhs i₁ i₂ → SimRel rel₂ lhs rhs i₁ i₂ := mono_rel (by simp)
+
+-- theorem SimRel.inf_iff [Determ Eq lhs] [Determ Eq rhs]
+--   : SimRel (rel₁ ⊓ rel₂) lhs rhs i₁ i₂
+--     ↔ SimRel rel₁ lhs rhs i₁ i₂ ∧ SimRel rel₂ lhs rhs i₁ i₂ :=
+--   ⟨fun h => ⟨lhs_of_inf h, rhs_of_inf h⟩,
+--    fun ⟨h1, h2⟩ => inf h1 h2⟩
+
+-- -- TODO: need inhabitance...
+-- theorem SimRelUpto.refl
+--   {rel} [IsRefl α rel]
+--   {addr : ι → Node α ι → Prop} [InhabAt ⊤ addr]
+--   {gas} (i) : SimRelUpto ⊤ rel addr addr gas i i
+--   := match gas with
+--   | 0 => .done i i trivial
+--   | _ + 1 =>
+--     have ⟨y, hy⟩ := rel_inhab addr i;
+--     .node hy hy (IsRefl.refl _) rfl (fun j => refl (getChild y j))
+
+-- theorem SimRel.refl
+--   {rel} [IsRefl α rel] {addr : ι → Node α ι → Prop} [InhabAt ⊤ addr] (i)
+--    : SimRel rel addr addr i i
+--   := fun _ => .refl i
+
+-- theorem SimRelUpto.symm {rel} [IsSymm α rel]
+--   {lhs : ι₁ → Node α ι₁ → Prop} {rhs : ι₂ → Node α ι₂ → Prop}
+--   {gas} {i₁ i₂}
+--   : SimRelUpto stop rel lhs rhs gas i₁ i₂ → SimRelUpto stop rel rhs lhs gas i₂ i₁
+--   | .done _ _ hs => .done i₂ i₁ hs
 --   | .node hn₁ hn₂ h_tag h_numChildren h_children =>
---     .node hn₁ hn₂ ⟨h_tag⟩ h_numChildren (fun j => fin_sim (h_children j))
+--     .node hn₂ hn₁ (IsSymm.symm _ _ h_tag) h_numChildren.symm
+--       (fun j => symm (h_children (j.cast (Eq.symm h_numChildren))))
 
--- theorem EFinTrace.sim
---   : EFinTrace data lhs rhs i₁ i₂ → SimRel (fun x y => Nonempty (data x y)) lhs rhs i₁ i₂ :=
---   fun t => (t.fin_sim).sim
+-- theorem SimRel.symm {rel} [IsSymm α rel]
+--   {lhs : ι₁ → Node α ι₁ → Prop} {rhs : ι₂ → Node α ι₂ → Prop}
+--   {i₁ i₂}
+--   (h : SimRel rel lhs rhs i₁ i₂) : SimRel rel rhs lhs i₂ i₁
+--   := fun n => (h n).symm
 
-theorem SimRelUpto.notBot : SimRelUpto stop ⊥ lhs rhs (gas + 1) i₁ i₂ → False
-  | .node _ _ h_tag _ _ => by cases h_tag
+-- theorem SimRelUpto.gtrans
+--   {α β γ} [BinderList α] [BinderList β] [BinderList γ]
+--   {rel₁ : α → β → Prop} {rel₂ : β → γ → Prop} {rel₃ : α → γ → Prop}
+--   (hrel : ∀ a b c, rel₁ a b → rel₂ b c → rel₃ a c)
+--   {ι₁ ι₂ ι₃}
+--   {lhs : ι₁ → Node α ι₁ → Prop} {mid : ι₂ → Node β ι₂ → Prop} {rhs : ι₃ → Node γ ι₃ → Prop}
+--   [Determ Eq lhs] [Determ Eq mid] [Determ Eq rhs]
+--   {gas} {i₁ i₂ i₃}
+--   : SimRelUpto stop rel₁ lhs mid gas i₁ i₂ → SimRelUpto stop rel₂ mid rhs gas i₂ i₃
+--     → SimRelUpto stop rel₃ lhs rhs gas i₁ i₃
+--   | .done _ _ hs, .done _ _ _ => .done i₁ i₃ hs
+--   | .node hn₁ hn₂ h1_tag h1_numChildren h1_children,
+--     .node hn₂' hn₃ h2_tag h2_numChildren h2_children => by
+--     cases determ_eq hn₂ hn₂'
+--     exact .node hn₁ hn₃ (hrel _ _ _ h1_tag h2_tag) (h1_numChildren.trans h2_numChildren)
+--       (fun j => gtrans hrel (h1_children j) (h2_children (j.cast h1_numChildren)))
 
-theorem SimRelUpto.ne_bot (h : SimRelUpto stop rel lhs rhs (gas + 1) i₁ i₂) : rel ≠ ⊥
-  := fun e => (e ▸ h).notBot
+-- theorem SimRel.gtrans
+--   {α β γ} [BinderList α] [BinderList β] [BinderList γ]
+--   {rel₁ : α → β → Prop} {rel₂ : β → γ → Prop} {rel₃ : α → γ → Prop}
+--   (hrel : ∀ a b c, rel₁ a b → rel₂ b c → rel₃ a c)
+--   {ι₁ ι₂ ι₃}
+--   {lhs : ι₁ → Node α ι₁ → Prop} {mid : ι₂ → Node β ι₂ → Prop} {rhs : ι₃ → Node γ ι₃ → Prop}
+--   [Determ Eq lhs] [Determ Eq mid] [Determ Eq rhs]
+--   {i₁ i₂ i₃}
+--   (h1 : SimRel rel₁ lhs mid i₁ i₂)
+--   (h2 : SimRel rel₂ mid rhs i₂ i₃)
+--   : SimRel rel₃ lhs rhs i₁ i₃
+--   := fun n => SimRelUpto.gtrans hrel (h1 n) (h2 n)
 
-theorem SimRel.notBot (h : SimRel ⊥ lhs rhs i₁ i₂) : False := (h 1).notBot
-
-theorem SimRel.ne_bot (h : SimRel rel lhs rhs i₁ i₂) : rel ≠ ⊥ := (h 1).ne_bot
-
-theorem FinSimRel.notBot : FinSimRel ⊥ lhs rhs i₁ i₂ → False
-  := fun ⟨gas + 1, .node _ _ h_tag _ _⟩ => by cases h_tag
-
-theorem FinSimRel.ne_bot (h : FinSimRel rel lhs rhs i₁ i₂) : rel ≠ ⊥
-  := fun e => (e ▸ h).notBot
-
-theorem SimRelUpto.mono_rel (hrel : rel₁ ≤ rel₂) {gas} {i₁ : ι₁} {i₂ : ι₂}
-  : SimRelUpto stop rel₁ lhs rhs gas i₁ i₂ → SimRelUpto stop rel₂ lhs rhs gas i₁ i₂
-  | .done _ _ hs => .done i₁ i₂ hs
-  | .node hn₁ hn₂ h_tag h_numChildren h_children =>
-    .node hn₁ hn₂ (hrel _ _ h_tag) h_numChildren (fun j => mono_rel hrel (h_children j))
-
-theorem SimRel.mono_rel (hrel : rel₁ ≤ rel₂) {i₁ : ι₁} {i₂ : ι₂} (h : SimRel rel₁ lhs rhs i₁ i₂)
-  : SimRel rel₂ lhs rhs i₁ i₂ := fun n => (h n).mono_rel hrel
-
-theorem SimRelUpto.inf [Determ Eq lhs] [Determ Eq rhs] {gas} {i₁ : ι₁} {i₂ : ι₂}
-  : SimRelUpto stop rel₁ lhs rhs gas i₁ i₂
-  → SimRelUpto stop rel₂ lhs rhs gas i₁ i₂
-  → SimRelUpto stop (rel₁ ⊓ rel₂) lhs rhs gas i₁ i₂
-  | .done _ _ hs,
-    .done _ _ _ => .done i₁ i₂ hs
-  | .node hn₁ hn₂ h1_tag h1_numChildren h1_children,
-    .node hn₁' hn₂' h2_tag _ h2_children => by
-    cases determ_eq hn₁ hn₁'
-    cases determ_eq hn₂ hn₂'
-    exact .node (rel := rel₁ ⊓ rel₂)
-      hn₁ hn₂
-      (And.intro h1_tag h2_tag) h1_numChildren
-      (fun j => SimRelUpto.inf (h1_children j) (h2_children j))
-
-theorem SimRel.inf [Determ Eq lhs] [Determ Eq rhs] {i₁ : ι₁} {i₂ : ι₂}
-  (h₁ : SimRel rel₁ lhs rhs i₁ i₂)
-  (h₂ : SimRel rel₂ lhs rhs i₁ i₂) : SimRel (rel₁ ⊓ rel₂) lhs rhs i₁ i₂ :=
-  fun n => SimRelUpto.inf (h₁ n) (h₂ n)
-
-theorem SimRelUpto.lhs_of_inf
-  : SimRelUpto stop (rel₁ ⊓ rel₂) lhs rhs gas i₁ i₂ → SimRelUpto stop rel₁ lhs rhs gas i₁ i₂
-  := mono_rel (by simp)
-
-theorem SimRelUpto.rhs_of_inf
-  : SimRelUpto stop (rel₁ ⊓ rel₂) lhs rhs gas i₁ i₂ → SimRelUpto stop rel₂ lhs rhs gas i₁ i₂
-  := mono_rel (by simp)
-
-theorem SimRelUpto.inf_iff [Determ Eq lhs] [Determ Eq rhs]
-  : SimRelUpto stop (rel₁ ⊓ rel₂) lhs rhs gas i₁ i₂
-    ↔ SimRelUpto stop rel₁ lhs rhs gas i₁ i₂ ∧ SimRelUpto stop rel₂ lhs rhs gas i₁ i₂ :=
-  ⟨fun h => ⟨lhs_of_inf h, rhs_of_inf h⟩,
-   fun ⟨h1, h2⟩ => inf h1 h2⟩
-
-theorem SimRel.lhs_of_inf
-  : SimRel (rel₁ ⊓ rel₂) lhs rhs i₁ i₂ → SimRel rel₁ lhs rhs i₁ i₂ := mono_rel (by simp)
-
-theorem SimRel.rhs_of_inf
-  : SimRel (rel₁ ⊓ rel₂) lhs rhs i₁ i₂ → SimRel rel₂ lhs rhs i₁ i₂ := mono_rel (by simp)
-
-theorem SimRel.inf_iff [Determ Eq lhs] [Determ Eq rhs]
-  : SimRel (rel₁ ⊓ rel₂) lhs rhs i₁ i₂
-    ↔ SimRel rel₁ lhs rhs i₁ i₂ ∧ SimRel rel₂ lhs rhs i₁ i₂ :=
-  ⟨fun h => ⟨lhs_of_inf h, rhs_of_inf h⟩,
-   fun ⟨h1, h2⟩ => inf h1 h2⟩
-
--- TODO: need inhabitance...
-theorem SimRelUpto.refl
-  {rel} [IsRefl α rel]
-  {addr : ι → Node α ι → Prop} [InhabAt ⊤ addr]
-  {gas} (i) : SimRelUpto ⊤ rel addr addr gas i i
-  := match gas with
-  | 0 => .done i i trivial
-  | _ + 1 =>
-    have ⟨y, hy⟩ := rel_inhab addr i;
-    .node hy hy (IsRefl.refl _) rfl (fun j => refl (getChild y j))
-
-theorem SimRel.refl
-  {rel} [IsRefl α rel] {addr : ι → Node α ι → Prop} [InhabAt ⊤ addr] (i) : SimRel rel addr addr i i
-  := fun _ => .refl i
-
-theorem SimRelUpto.symm {rel} [IsSymm α rel]
-  {lhs : ι₁ → Node α ι₁ → Prop} {rhs : ι₂ → Node α ι₂ → Prop}
-  {gas} {i₁ i₂}
-  : SimRelUpto stop rel lhs rhs gas i₁ i₂ → SimRelUpto stop rel rhs lhs gas i₂ i₁
-  | .done _ _ hs => .done i₂ i₁ hs
-  | .node hn₁ hn₂ h_tag h_numChildren h_children =>
-    .node hn₂ hn₁ (IsSymm.symm _ _ h_tag) h_numChildren.symm
-      (fun j => symm (h_children (j.cast (Eq.symm h_numChildren))))
-
-theorem SimRel.symm {rel} [IsSymm α rel]
-  {lhs : ι₁ → Node α ι₁ → Prop} {rhs : ι₂ → Node α ι₂ → Prop}
-  {i₁ i₂}
-  (h : SimRel rel lhs rhs i₁ i₂) : SimRel rel rhs lhs i₂ i₁
-  := fun n => (h n).symm
-
-theorem SimRelUpto.gtrans
-  {α β γ} [BinderList α] [BinderList β] [BinderList γ]
-  {rel₁ : α → β → Prop} {rel₂ : β → γ → Prop} {rel₃ : α → γ → Prop}
-  (hrel : ∀ a b c, rel₁ a b → rel₂ b c → rel₃ a c)
-  {ι₁ ι₂ ι₃}
-  {lhs : ι₁ → Node α ι₁ → Prop} {mid : ι₂ → Node β ι₂ → Prop} {rhs : ι₃ → Node γ ι₃ → Prop}
-  [Determ Eq lhs] [Determ Eq mid] [Determ Eq rhs]
-  {gas} {i₁ i₂ i₃}
-  : SimRelUpto stop rel₁ lhs mid gas i₁ i₂ → SimRelUpto stop rel₂ mid rhs gas i₂ i₃
-    → SimRelUpto stop rel₃ lhs rhs gas i₁ i₃
-  | .done _ _ hs, .done _ _ _ => .done i₁ i₃ hs
-  | .node hn₁ hn₂ h1_tag h1_numChildren h1_children,
-    .node hn₂' hn₃ h2_tag h2_numChildren h2_children => by
-    cases determ_eq hn₂ hn₂'
-    exact .node hn₁ hn₃ (hrel _ _ _ h1_tag h2_tag) (h1_numChildren.trans h2_numChildren)
-      (fun j => gtrans hrel (h1_children j) (h2_children (j.cast h1_numChildren)))
-
-theorem SimRel.gtrans
-  {α β γ} [BinderList α] [BinderList β] [BinderList γ]
-  {rel₁ : α → β → Prop} {rel₂ : β → γ → Prop} {rel₃ : α → γ → Prop}
-  (hrel : ∀ a b c, rel₁ a b → rel₂ b c → rel₃ a c)
-  {ι₁ ι₂ ι₃}
-  {lhs : ι₁ → Node α ι₁ → Prop} {mid : ι₂ → Node β ι₂ → Prop} {rhs : ι₃ → Node γ ι₃ → Prop}
-  [Determ Eq lhs] [Determ Eq mid] [Determ Eq rhs]
-  {i₁ i₂ i₃}
-  (h1 : SimRel rel₁ lhs mid i₁ i₂)
-  (h2 : SimRel rel₂ mid rhs i₂ i₃)
-  : SimRel rel₃ lhs rhs i₁ i₃
-  := fun n => SimRelUpto.gtrans hrel (h1 n) (h2 n)
-
-theorem SimRelUpto.trans {rel} [IsTrans α rel]
-  {ι₁ ι₂ ι₃}
-  {lhs : ι₁ → Node α ι₁ → Prop} {mid : ι₂ → Node α ι₂ → Prop} {rhs : ι₃ → Node α ι₃ → Prop}
-  [Determ Eq lhs] [Determ Eq mid] [Determ Eq rhs]
-  {gas} {i₁ i₂ i₃}
-  (h1 : SimRelUpto stop rel lhs mid gas i₁ i₃)
-  (h2 : SimRelUpto stop rel mid rhs gas i₃ i₂)
-  : SimRelUpto stop rel lhs rhs gas i₁ i₂
-  := h1.gtrans IsTrans.trans h2
-
-theorem SimRel.trans {rel} [IsTrans α rel]
-  {ι₁ ι₂ ι₃}
-  {lhs : ι₁ → Node α ι₁ → Prop} {mid : ι₂ → Node α ι₂ → Prop} {rhs : ι₃ → Node α ι₃ → Prop}
-  [Determ Eq lhs] [Determ Eq mid] [Determ Eq rhs]
-  {i₁ i₂ i₃}
-  (h1 : SimRel rel lhs mid i₁ i₃)
-  (h2 : SimRel rel mid rhs i₃ i₂)
-  : SimRel rel lhs rhs i₁ i₂
-  := h1.gtrans IsTrans.trans h2
-
--- theorem SimRelUpto.map_lhs
---   {ι₁'} (map : ι₁ → ι₁' → Prop) [InhabAt ⊤ map]
---   {gas} {i₁ i₂ i₁'} (hi' : map i₁ i₁')
+-- theorem SimRelUpto.trans {rel} [IsTrans α rel]
+--   {ι₁ ι₂ ι₃}
+--   {lhs : ι₁ → Node α ι₁ → Prop} {mid : ι₂ → Node α ι₂ → Prop} {rhs : ι₃ → Node α ι₃ → Prop}
+--   [Determ Eq lhs] [Determ Eq mid] [Determ Eq rhs]
+--   {gas} {i₁ i₂ i₃}
+--   (h1 : SimRelUpto stop rel lhs mid gas i₁ i₃)
+--   (h2 : SimRelUpto stop rel mid rhs gas i₃ i₂)
 --   : SimRelUpto stop rel lhs rhs gas i₁ i₂
---   → SimRelUpto stop rel (fun x y => ∃x', lhs (f x) (y.mapChildren f)) rhs gas i' i₂
---   | .done _ _ hs => .done _ _ hs
---   | .node hn₁ hn₂ h_tag h_numChildren h_children =>
---     .node (lhs := fun x y => lhs (f x) (y.mapChildren f)) sorry hn₂ h_tag h_numChildren
---       (fun j => map_lhs f _ sorry sorry)
+--   := h1.gtrans IsTrans.trans h2
 
--- theorem SimRel.map_lhs
---   {ι'} (f : ι' → ι₁)
---   {i₁ i₂} (i') (hi' : f i' = i₁)
---   : SimRel rel lhs rhs i₁ i₂ → SimRel rel (fun x y => lhs (f x) (y.mapChildren f)) rhs i' i₂
---   := sorry
+-- theorem SimRel.trans {rel} [IsTrans α rel]
+--   {ι₁ ι₂ ι₃}
+--   {lhs : ι₁ → Node α ι₁ → Prop} {mid : ι₂ → Node α ι₂ → Prop} {rhs : ι₃ → Node α ι₃ → Prop}
+--   [Determ Eq lhs] [Determ Eq mid] [Determ Eq rhs]
+--   {i₁ i₂ i₃}
+--   (h1 : SimRel rel lhs mid i₁ i₃)
+--   (h2 : SimRel rel mid rhs i₃ i₂)
+--   : SimRel rel lhs rhs i₁ i₂
+--   := h1.gtrans IsTrans.trans h2
 
-end Node
+-- -- theorem SimRelUpto.map_lhs
+-- --   {ι₁'} (map : ι₁ → ι₁' → Prop) [InhabAt ⊤ map]
+-- --   {gas} {i₁ i₂ i₁'} (hi' : map i₁ i₁')
+-- --   : SimRelUpto stop rel lhs rhs gas i₁ i₂
+-- --   → SimRelUpto stop rel (fun x y => ∃x', lhs (f x) (y.mapChildren f)) rhs gas i' i₂
+-- --   | .done _ _ hs => .done _ _ hs
+-- --   | .node hn₁ hn₂ h_tag h_numChildren h_children =>
+-- --     .node (lhs := fun x y => lhs (f x) (y.mapChildren f)) sorry hn₂ h_tag h_numChildren
+-- --       (fun j => map_lhs f _ sorry sorry)
 
-end SimRel
+-- -- theorem SimRel.map_lhs
+-- --   {ι'} (f : ι' → ι₁)
+-- --   {i₁ i₂} (i') (hi' : f i' = i₁)
+-- --   : SimRel rel lhs rhs i₁ i₂ → SimRel rel (fun x y => lhs (f x) (y.mapChildren f)) rhs i' i₂
+-- --   := sorry
 
-section Sim
+-- end Node
 
-variable {stop : Prop} {α β} [BinderList α] [BinderList β]
-        {data data₁ data₂ : α → β → Type _}
-        {rel rel₁ : α → β → Prop}
-        {ι₁ ι₂ ι₁' ι₂'}
-        {lhs : ι₁ → Node α ι₁} {rhs : ι₂ → Node β ι₂}
-        {i₁ : ι₁} {i₂ : ι₂} {n₁ n₂}
+-- end SimRel
 
--- TODO: map things using injections
+-- section Sim
 
--- TODO: such mappings give us ≈ objects...
+-- variable {stop : Prop} {α β} [BinderList α] [BinderList β]
+--         {data data₁ data₂ : α → β → Type _}
+--         {rel rel₁ : α → β → Prop}
+--         {ι₁ ι₂ ι₁' ι₂'}
+--         {lhs : ι₁ → Node α ι₁} {rhs : ι₂ → Node β ι₂}
+--         {i₁ : ι₁} {i₂ : ι₂} {n₁ n₂}
 
--- TODO: letting us play ℕ games to build cotrees out of trees!
+-- -- TODO: map things using injections
 
-namespace Node
+-- -- TODO: such mappings give us ≈ objects...
 
-theorem SimUpto.map_lhs {gas}
-  {i₁ i₂} (f : ι₁ → ι₁') (g : ι₁' → ι₁)
-  (hfg : ∀ i, g (f i) = i)
-  : SimUpto stop rel lhs rhs gas i₁ i₂
-  → SimUpto stop rel (Node.mapChildren f ∘ lhs ∘ g) rhs gas (f i₁) i₂
-  | .done _ _ hs => .done (f i₁) i₂ hs
-  | .node (n₁ := n₁) hn₁ hn₂ h_tag h_numChildren h_children =>
-    .node (lhs := readMem (Node.mapChildren f ∘ lhs ∘ g))
-          (rhs := readMem rhs)
-          (n₁ := n₁.mapChildren f)
-          (by simp only [hfg, implies_true, readMem, Function.comp_apply] at *; rw [hn₁]) hn₂
-          (by simp [mapChildren, h_tag]) (by simp [mapChildren, h_numChildren])
-          (fun j => map_lhs f g hfg (h_children j))
+-- -- TODO: letting us play ℕ games to build cotrees out of trees!
 
-theorem SimUpto.map_rhs {gas}
-  {i₁ i₂} (f : ι₂ → ι₂') (g : ι₂' → ι₂)
-  (hfg : ∀ i, g (f i) = i)
-  : SimUpto stop rel lhs rhs gas i₁ i₂
-  → SimUpto stop rel lhs (Node.mapChildren f ∘ rhs ∘ g) gas i₁ (f i₂)
-  | .done _ _ hs => .done i₁ (f i₂) hs
-  | .node (n₂ := n₂) hn₁ hn₂ h_tag h_numChildren h_children =>
-    .node (lhs := readMem lhs)
-          (rhs := readMem (Node.mapChildren f ∘ rhs ∘ g))
-          (n₂ := n₂.mapChildren f)
-          hn₁
-          (by simp only [hfg, implies_true, readMem, Function.comp_apply] at *; rw [hn₂])
-          (by simp [mapChildren, h_tag]) (by simp [mapChildren, h_numChildren])
-          (fun j => map_rhs f g hfg (h_children j))
+-- namespace Node
 
-theorem SimUpto.map_both
-  {gas} {ι ι'} (f : ι → ι') (g : ι' → ι)
-  (hfg : ∀ i, g (f i) = i)
-  {lhs : ι → Node α ι}
-  {rhs : ι → Node β ι}
-  {i₁ i₂}
-  : SimUpto stop rel lhs rhs gas i₁ i₂
-  → SimUpto stop rel (Node.mapChildren f ∘ lhs ∘ g) (Node.mapChildren f ∘ rhs ∘ g) gas (f i₁) (f i₂)
-  := fun h => (h.map_lhs f g hfg).map_rhs f g hfg
+-- theorem SimUpto.map_lhs {gas}
+--   {i₁ i₂} (f : ι₁ → ι₁') (g : ι₁' → ι₁)
+--   (hfg : ∀ i, g (f i) = i)
+--   : SimUpto stop rel lhs rhs gas i₁ i₂
+--   → SimUpto stop rel (Node.mapChildren f ∘ lhs ∘ g) rhs gas (f i₁) i₂
+--   | .done _ _ hs => .done (f i₁) i₂ hs
+--   | .node (n₁ := n₁) hn₁ hn₂ h_tag h_numChildren h_children =>
+--     .node (lhs := readMem (Node.mapChildren f ∘ lhs ∘ g))
+--           (rhs := readMem rhs)
+--           (n₁ := n₁.mapChildren f)
+--           (by simp only [hfg, implies_true, readMem, Function.comp_apply] at *; rw [hn₁]) hn₂
+--           (by simp [mapChildren, h_tag]) (by simp [mapChildren, h_numChildren])
+--           (fun j => map_lhs f g hfg (h_children j))
 
-theorem Sim.map_lhs
-  {ι₁'} (f : ι₁ → ι₁') (g : ι₁' → ι₁)
-  (hfg : ∀ i, g (f i) = i)
-  {i₁ i₂}
-  : Sim rel lhs rhs i₁ i₂
-  → Sim rel (Node.mapChildren f ∘ lhs ∘ g) rhs (f i₁) i₂
-  := fun h n => SimUpto.map_lhs f g hfg (h n)
+-- theorem SimUpto.map_rhs {gas}
+--   {i₁ i₂} (f : ι₂ → ι₂') (g : ι₂' → ι₂)
+--   (hfg : ∀ i, g (f i) = i)
+--   : SimUpto stop rel lhs rhs gas i₁ i₂
+--   → SimUpto stop rel lhs (Node.mapChildren f ∘ rhs ∘ g) gas i₁ (f i₂)
+--   | .done _ _ hs => .done i₁ (f i₂) hs
+--   | .node (n₂ := n₂) hn₁ hn₂ h_tag h_numChildren h_children =>
+--     .node (lhs := readMem lhs)
+--           (rhs := readMem (Node.mapChildren f ∘ rhs ∘ g))
+--           (n₂ := n₂.mapChildren f)
+--           hn₁
+--           (by simp only [hfg, implies_true, readMem, Function.comp_apply] at *; rw [hn₂])
+--           (by simp [mapChildren, h_tag]) (by simp [mapChildren, h_numChildren])
+--           (fun j => map_rhs f g hfg (h_children j))
 
-theorem Sim.map_rhs
-  {ι₂'} (f : ι₂ → ι₂') (g : ι₂' → ι₂)
-  (hfg : ∀ i, g (f i) = i)
-  {i₁ i₂}
-  : Sim rel lhs rhs i₁ i₂
-  → Sim rel lhs (Node.mapChildren f ∘ rhs ∘ g) i₁ (f i₂)
-  := fun h n => SimUpto.map_rhs f g hfg (h n)
+-- theorem SimUpto.map_both
+--   {gas} {ι ι'} (f : ι → ι') (g : ι' → ι)
+--   (hfg : ∀ i, g (f i) = i)
+--   {lhs : ι → Node α ι}
+--   {rhs : ι → Node β ι}
+--   {i₁ i₂}
+--   : SimUpto stop rel lhs rhs gas i₁ i₂
+--   → SimUpto stop rel
+--      (Node.mapChildren f ∘ lhs ∘ g) (Node.mapChildren f ∘ rhs ∘ g) gas (f i₁) (f i₂)
+--   := fun h => (h.map_lhs f g hfg).map_rhs f g hfg
 
-theorem Sim.map_both
-  {ι ι'} (f : ι → ι') (g : ι' → ι)
-  (hfg : ∀ i, g (f i) = i)
-  {lhs : ι → Node α ι} {rhs : ι → Node β ι}
-  {i₁ i₂}
-  : Sim rel lhs rhs i₁ i₂
-  → Sim rel (Node.mapChildren f ∘ lhs ∘ g) (Node.mapChildren f ∘ rhs ∘ g) (f i₁) (f i₂)
-  := fun h n => SimUpto.map_both f g hfg (h n)
+-- theorem Sim.map_lhs
+--   {ι₁'} (f : ι₁ → ι₁') (g : ι₁' → ι₁)
+--   (hfg : ∀ i, g (f i) = i)
+--   {i₁ i₂}
+--   : Sim rel lhs rhs i₁ i₂
+--   → Sim rel (Node.mapChildren f ∘ lhs ∘ g) rhs (f i₁) i₂
+--   := fun h n => SimUpto.map_lhs f g hfg (h n)
 
-end Node
+-- theorem Sim.map_rhs
+--   {ι₂'} (f : ι₂ → ι₂') (g : ι₂' → ι₂)
+--   (hfg : ∀ i, g (f i) = i)
+--   {i₁ i₂}
+--   : Sim rel lhs rhs i₁ i₂
+--   → Sim rel lhs (Node.mapChildren f ∘ rhs ∘ g) i₁ (f i₂)
+--   := fun h n => SimUpto.map_rhs f g hfg (h n)
 
-end Sim
+-- theorem Sim.map_both
+--   {ι ι'} (f : ι → ι') (g : ι' → ι)
+--   (hfg : ∀ i, g (f i) = i)
+--   {lhs : ι → Node α ι} {rhs : ι → Node β ι}
+--   {i₁ i₂}
+--   : Sim rel lhs rhs i₁ i₂
+--   → Sim rel (Node.mapChildren f ∘ lhs ∘ g) (Node.mapChildren f ∘ rhs ∘ g) (f i₁) (f i₂)
+--   := fun h n => SimUpto.map_both f g hfg (h n)
+
+-- end Node
+
+-- end Sim
 
 /-- A pre-cotree over a given address space -/
 structure PCotree (ι : Type _) (α : Type _) [NumChildren α] : Type _ where
@@ -431,25 +433,25 @@ instance PCotree.instFlatChildren {ι α} [BinderList α]
 
 def PCotree.Sim {ι₁ ι₂ α β} [BinderList α] [BinderList β] (rel : α → β → Prop)
   (t₁ : PCotree ι₁ α) (t₂ : PCotree ι₂ β) : Prop
-  := Node.Sim rel t₁.getNode t₂.getNode t₁.ix t₂.ix
+  := SimIxRel rel t₁.getNode t₂.getNode t₁.ix t₂.ix
 
 theorem PCotree.Sim.refl {ι α} [BinderList α]
   {rel} [IsRefl α rel]
   (t : PCotree ι α) : PCotree.Sim rel t t :=
-  Node.SimRel.refl t.ix
+  SimIxRel.refl t.ix
 
 theorem PCotree.Sim.symm {ι₁ ι₂ α} [BinderList α]
   {rel} [IsSymm α rel]
   {t₁ : PCotree ι₁ α} {t₂ : PCotree ι₂ α}
   (h : PCotree.Sim rel t₁ t₂) : PCotree.Sim rel t₂ t₁ :=
-  Node.SimRel.symm h
+  SimIxRel.symm h
 
 theorem PCotree.Sim.trans {ι₁ ι₂ ι₃ α} [BinderList α]
   {rel} [IsTrans α rel]
   {t₁ : PCotree ι₁ α} {t₂ : PCotree ι₂ α} {t₃ : PCotree ι₃ α}
   (h1 : PCotree.Sim rel t₁ t₂)
   (h2 : PCotree.Sim rel t₂ t₃) : PCotree.Sim rel t₁ t₃ :=
-  Node.SimRel.trans h1 h2
+  SimIxRel.trans h1 h2
 
 theorem PCotree.Sim.tag {ι₁ ι₂ α β} [BinderList α] [BinderList β]
   {rel} {t₁ : PCotree ι₁ α} {t₂ : PCotree ι₂ β}
@@ -457,46 +459,43 @@ theorem PCotree.Sim.tag {ι₁ ι₂ α β} [BinderList α] [BinderList β]
   let hsim := h 1
   match hsim with
   | .node hn₁ hn₂ h_tag _ _ => by
-    cases determ_eq hn₁ (readMem.refl t₁.getNode t₁.ix);
-    cases determ_eq hn₂ (readMem.refl t₂.getNode t₂.ix);
+    cases hn₁; cases hn₂;
     exact h_tag
 
-theorem PCotree.Sim.numChildren {ι₁ ι₂ α β} [BinderList α] [BinderList β]
-  {rel} {t₁ : PCotree ι₁ α} {t₂ : PCotree ι₂ β}
-  (h : PCotree.Sim rel t₁ t₂) : numChildren t₁ = numChildren t₂ :=
-  let hsim := h 1
-  match hsim with
-  | .node hn₁ hn₂ h_tag h_numChildren _ => by
-    cases determ_eq hn₁ (readMem.refl t₁.getNode t₁.ix);
-    cases determ_eq hn₂ (readMem.refl t₂.getNode t₂.ix);
-    exact h_numChildren
+-- theorem PCotree.Sim.numChildren {ι₁ ι₂ α β} [BinderList α] [BinderList β]
+--   {rel} {t₁ : PCotree ι₁ α} {t₂ : PCotree ι₂ β}
+--   (h : PCotree.Sim rel t₁ t₂) : numChildren t₁ = numChildren t₂ :=
+--   let hsim := h 1
+--   match hsim with
+--   | .node hn₁ hn₂ h_tag h_numChildren _ => by
+--     cases hn₁; cases hn₂;
+--     exact h_numChildren
 
-theorem PCotree.Sim.childrenIx {ι₁ ι₂ α β} [BinderList α] [BinderList β]
-  {rel} {t₁ : PCotree ι₁ α} {t₂ : PCotree ι₂ β}
-  (h : PCotree.Sim rel t₁ t₂) (j) :
-  Node.Sim rel t₁.getNode t₂.getNode
-    (getChild t₁ j) (getChild t₂ (j.cast (PCotree.Sim.numChildren h)))
-  := fun n =>
-    let hsim := h (n + 1)
-    match hsim with
-    | .node hn₁ hn₂ h_tag h_numChildren h_children => by
-      cases determ_eq hn₁ (readMem.refl t₁.getNode t₁.ix);
-      cases determ_eq hn₂ (readMem.refl t₂.getNode t₂.ix);
-      exact h_children j
+-- theorem PCotree.Sim.childrenIx {ι₁ ι₂ α β} [BinderList α] [BinderList β]
+--   {rel} {t₁ : PCotree ι₁ α} {t₂ : PCotree ι₂ β}
+--   (h : PCotree.Sim rel t₁ t₂) (j) :
+--   Sim rel t₁.getNode t₂.getNode
+--     (getChild t₁ j) (getChild t₂ (j.cast (PCotree.Sim.numChildren h)))
+--   := fun n =>
+--     let hsim := h (n + 1)
+--     match hsim with
+--     | .node hn₁ hn₂ h_tag h_numChildren h_children => by
+--       cases hn₁; cases hn₂;
+--       exact h_children j
 
-theorem PCotree.Sim.children {ι₁ ι₂ α β} [BinderList α] [BinderList β]
-  {rel} {t₁ : PCotree ι₁ α} {t₂ : PCotree ι₂ β}
-  (h : PCotree.Sim rel t₁ t₂) (j) :
-  PCotree.Sim rel
-    (getChild (β := PCotree ι₁ α) t₁ j)
-    (getChild (β := PCotree ι₂ β) t₂ (j.cast (PCotree.Sim.numChildren h)))
-  := fun n =>
-    let hsim := h (n + 1)
-    match hsim with
-    | .node hn₁ hn₂ h_tag h_numChildren h_children => by
-      cases determ_eq hn₁ (readMem.refl t₁.getNode t₁.ix);
-      cases determ_eq hn₂ (readMem.refl t₂.getNode t₂.ix);
-      exact h_children j
+-- theorem PCotree.Sim.children {ι₁ ι₂ α β} [BinderList α] [BinderList β]
+--   {rel} {t₁ : PCotree ι₁ α} {t₂ : PCotree ι₂ β}
+--   (h : PCotree.Sim rel t₁ t₂) (j) :
+--   PCotree.Sim rel
+--     (getChild (β := PCotree ι₁ α) t₁ j)
+--     (getChild (β := PCotree ι₂ β) t₂ (j.cast (PCotree.Sim.numChildren h)))
+--   := fun n =>
+--     let hsim := h (n + 1)
+--     match hsim with
+--     | .node hn₁ hn₂ h_tag h_numChildren h_children => by
+--       cases determ_eq hn₁ (readMem.refl t₁.getNode t₁.ix);
+--       cases determ_eq hn₂ (readMem.refl t₂.getNode t₂.ix);
+--       exact h_children j
 
 instance PCotree.setoid (ι α) [BinderList α] : Setoid (PCotree ι α) where
   r := PCotree.Sim Eq
@@ -505,19 +504,19 @@ instance PCotree.setoid (ι α) [BinderList α] : Setoid (PCotree ι α) where
 theorem PCotree.eqv_tag {ι α} [BinderList α]
   {t₁ t₂ : PCotree ι α} (h : t₁ ≈ t₂) : t₁.tag = t₂.tag := Sim.tag h
 
-theorem PCotree.eqv_numChildren {ι α} [BinderList α]
-  {t₁ t₂ : PCotree ι α} (h : t₁ ≈ t₂) : numChildren t₁ = numChildren t₂ := Sim.numChildren h
+-- theorem PCotree.eqv_numChildren {ι α} [BinderList α]
+--   {t₁ t₂ : PCotree ι α} (h : t₁ ≈ t₂) : numChildren t₁ = numChildren t₂ := Sim.numChildren h
 
-theorem PCotree.eqv_childrenIx {ι α} [BinderList α]
-  {t₁ t₂ : PCotree ι α} (h : t₁ ≈ t₂) (j) :
-  Node.Sim Eq t₁.getNode t₂.getNode
-    (getChild t₁ j) (getChild t₂ (j.cast (PCotree.eqv_numChildren h)))
-  := Sim.childrenIx h j
+-- theorem PCotree.eqv_childrenIx {ι α} [BinderList α]
+--   {t₁ t₂ : PCotree ι α} (h : t₁ ≈ t₂) (j) :
+--   Node.Sim Eq t₁.getNode t₂.getNode
+--     (getChild t₁ j) (getChild t₂ (j.cast (PCotree.eqv_numChildren h)))
+--   := Sim.childrenIx h j
 
-theorem PCotree.eqv_children {ι α} [BinderList α]
-  {t₁ t₂ : PCotree ι α} (h : t₁ ≈ t₂) (j)
-  : (getChild (β := PCotree ι α) t₁ j) ≈ (getChild t₂ (j.cast (PCotree.eqv_numChildren h)))
-  := Sim.children h j
+-- theorem PCotree.eqv_children {ι α} [BinderList α]
+--   {t₁ t₂ : PCotree ι α} (h : t₁ ≈ t₂) (j)
+--   : (getChild (β := PCotree ι α) t₁ j) ≈ (getChild t₂ (j.cast (PCotree.eqv_numChildren h)))
+--   := Sim.children h j
 
 theorem PCotree.neZero {n} {α} [NumChildren α]
   (t : PCotree (Fin n) α) : NeZero n :=
@@ -531,33 +530,33 @@ def PCotree.mapIx {ι₁ ι₂ α} [NumChildren α]
   ix := f t.ix
   getNode i := (t.getNode (g i)).mapChildren f
 
-theorem PCotree.mapIx_sim_eq {ι₁ ι₂ α} [BinderList α]
-  (f : ι₁ → ι₂) (g : ι₂ → ι₁)
-  (hfg : ∀ i, g (f i) = i)
-  (t : PCotree ι₁ α) :
-  t.Sim Eq (t.mapIx f g) := by
-  exact Node.Sim.map_rhs f g hfg (Sim.refl t)
+-- theorem PCotree.mapIx_sim_eq {ι₁ ι₂ α} [BinderList α]
+--   (f : ι₁ → ι₂) (g : ι₂ → ι₁)
+--   (hfg : ∀ i, g (f i) = i)
+--   (t : PCotree ι₁ α) :
+--   t.Sim Eq (t.mapIx f g) := by
+--   exact Node.Sim.map_rhs f g hfg (Sim.refl t)
 
-theorem PCotree.mapIx_eqv {ι₁ ι₂ α} [BinderList α]
-  {f : ι₁ → ι₂} {g : ι₂ → ι₁}
-  (hfg : ∀ i, g (f i) = i)
-  {t t' : PCotree ι₁ α} (h : t ≈ t') :
-  (t.mapIx f g) ≈ (t'.mapIx f g)
-  := ((t.mapIx_sim_eq f g hfg).symm.trans h).trans (t'.mapIx_sim_eq f g hfg)
+-- theorem PCotree.mapIx_eqv {ι₁ ι₂ α} [BinderList α]
+--   {f : ι₁ → ι₂} {g : ι₂ → ι₁}
+--   (hfg : ∀ i, g (f i) = i)
+--   {t t' : PCotree ι₁ α} (h : t ≈ t') :
+--   (t.mapIx f g) ≈ (t'.mapIx f g)
+--   := ((t.mapIx_sim_eq f g hfg).symm.trans h).trans (t'.mapIx_sim_eq f g hfg)
 
 def PCotree.finToNat {n} {α} [NumChildren α] (t : PCotree (Fin n) α) : PCotree ℕ α
   := t.mapIx Fin.val (have _ := t.neZero; Fin.ofNat n)
 
-theorem PCotree.finToNat_sim_eq {n} {α} [BinderList α] (t : PCotree (Fin n) α) :
-  t.Sim Eq t.finToNat
-  :=
-  have _  := t.neZero;
-  PCotree.mapIx_sim_eq Fin.val (Fin.ofNat n) (fun i => by simp) t
+-- theorem PCotree.finToNat_sim_eq {n} {α} [BinderList α] (t : PCotree (Fin n) α) :
+--   t.Sim Eq t.finToNat
+--   :=
+--   have _  := t.neZero;
+--   PCotree.mapIx_sim_eq Fin.val (Fin.ofNat n) (fun i => by simp) t
 
-theorem PCotree.finToNat_eqv {n} {α} [BinderList α] {t t' : PCotree (Fin n) α} (h : t ≈ t') :
-  t.finToNat ≈ t'.finToNat :=
-  have _ := t.neZero;
-  PCotree.mapIx_eqv (fun i => by simp) h
+-- theorem PCotree.finToNat_eqv {n} {α} [BinderList α] {t t' : PCotree (Fin n) α} (h : t ≈ t') :
+--   t.finToNat ≈ t'.finToNat :=
+--   have _ := t.neZero;
+--   PCotree.mapIx_eqv (fun i => by simp) h
 
 --TODO: mapIx; mapIx
 
@@ -586,17 +585,17 @@ theorem PCotree.numChildren_toCotree {ι α} [BinderList α]
 theorem PCotree.numChildren_quot {ι α} [BinderList α]
   (t : PCotree ι α) : numChildren (α := Cotree ι α) ⟦t⟧ = numChildren t := rfl
 
-instance Cotree.instFlatChildren {ι α} [BinderList α]
-  : FlatChildren (Cotree ι α) (Cotree ι α) where
-  getDChild t := t.hrecOn (fun t j => PCotree.toCotree (getChild t j)) (
-    fun a b h => by
-      simp only [PCotree.numChildren_quot]
-      rw [Fin.heq_fun_iff]
-      · intro i
-        apply Quotient.sound
-        apply PCotree.eqv_children h i
-      apply PCotree.eqv_numChildren h
-  )
+-- instance Cotree.instFlatChildren {ι α} [BinderList α]
+--   : FlatChildren (Cotree ι α) (Cotree ι α) where
+--   getDChild t := t.hrecOn (fun t j => PCotree.toCotree (getChild t j)) (
+--     fun a b h => by
+--       simp only [PCotree.numChildren_quot]
+--       rw [Fin.heq_fun_iff]
+--       · intro i
+--         apply Quotient.sound
+--         apply PCotree.eqv_children h i
+--       apply PCotree.eqv_numChildren h
+--   )
 
 instance PCotree.instInhabited {ι α} [Inhabited α] [Inhabited ι] [BinderList α]
   : Inhabited (PCotree ι α) := ⟨default, fun _ => default⟩
@@ -607,132 +606,132 @@ instance Cotree.instInhabited {ι α} [Inhabited α] [Inhabited ι] [BinderList 
 theorem Cotree.neZero {n} {α} [BinderList α]
   (t : Cotree (Fin n) α) : NeZero n := by induction t using Quot.ind with | mk t => exact t.neZero
 
-def Cotree.mapIx {ι₁ ι₂ α} [BinderList α]
-  (f : ι₁ → ι₂) (g : ι₂ → ι₁) (hfg : ∀ i, g (f i) = i)
-  (t : Cotree ι₁ α) : Cotree ι₂ α :=
-  Quotient.liftOn t (fun t => (t.mapIx f g).toCotree) fun _ _ h
-    => Quotient.sound <| PCotree.mapIx_eqv hfg h
+-- def Cotree.mapIx {ι₁ ι₂ α} [BinderList α]
+--   (f : ι₁ → ι₂) (g : ι₂ → ι₁) (hfg : ∀ i, g (f i) = i)
+--   (t : Cotree ι₁ α) : Cotree ι₂ α :=
+--   Quotient.liftOn t (fun t => (t.mapIx f g).toCotree) fun _ _ h
+--     => Quotient.sound <| PCotree.mapIx_eqv hfg h
 
-@[simp]
-theorem Cotree.mapIx_self {ι α} [BinderList α]
-  (f g : ι → ι) (hfg : ∀ i, g (f i) = i)
-  (t : Cotree ι α) :
-  t.mapIx f g hfg = t := by induction t using Quot.ind with | mk t =>
-  exact Quotient.sound (PCotree.mapIx_sim_eq f g hfg t).symm
+-- @[simp]
+-- theorem Cotree.mapIx_self {ι α} [BinderList α]
+--   (f g : ι → ι) (hfg : ∀ i, g (f i) = i)
+--   (t : Cotree ι α) :
+--   t.mapIx f g hfg = t := by induction t using Quot.ind with | mk t =>
+--   exact Quotient.sound (PCotree.mapIx_sim_eq f g hfg t).symm
 
-def Cotree.finToNat {n} {α} [BinderList α] (t : Cotree (Fin n) α) : Cotree ℕ α :=
-  Quotient.liftOn t (fun t => t.finToNat.toCotree) fun _ _ h
-    => Quotient.sound <| PCotree.finToNat_eqv h
+-- def Cotree.finToNat {n} {α} [BinderList α] (t : Cotree (Fin n) α) : Cotree ℕ α :=
+--   Quotient.liftOn t (fun t => t.finToNat.toCotree) fun _ _ h
+--     => Quotient.sound <| PCotree.finToNat_eqv h
 
 /-- A pre-cotree over a given partial address space -/
 structure PCotree? (ι : Type _) (α : Type _) [NumChildren α] : Type _ where
   ix : ι
   getNode : ι → Option (Node α ι)
 
-def PCotree?.Sim? {ι₁ ι₂ α β} [BinderList α] [BinderList β] (rel : α → β → Prop)
-  (t₁ : PCotree? ι₁ α) (t₂ : PCotree? ι₂ β) : Prop
-  := Node.Sim? rel t₁.getNode t₂.getNode t₁.ix t₂.ix
+-- def PCotree?.Sim? {ι₁ ι₂ α β} [BinderList α] [BinderList β] (rel : α → β → Prop)
+--   (t₁ : PCotree? ι₁ α) (t₂ : PCotree? ι₂ β) : Prop
+--   := Node.Sim? rel t₁.getNode t₂.getNode t₁.ix t₂.ix
 
-theorem PCotree?.Sim?.symm {ι₁ ι₂ α} [BinderList α]
-  {rel} [IsSymm α rel]
-  {t₁ : PCotree? ι₁ α} {t₂ : PCotree? ι₂ α}
-  (h : PCotree?.Sim? rel t₁ t₂) : PCotree?.Sim? rel t₂ t₁ :=
-  Node.SimRel.symm h
+-- theorem PCotree?.Sim?.symm {ι₁ ι₂ α} [BinderList α]
+--   {rel} [IsSymm α rel]
+--   {t₁ : PCotree? ι₁ α} {t₂ : PCotree? ι₂ α}
+--   (h : PCotree?.Sim? rel t₁ t₂) : PCotree?.Sim? rel t₂ t₁ :=
+--   Node.SimRel.symm h
 
-theorem PCotree?.Sim?.trans {ι₁ ι₂ ι₃ α} [BinderList α]
-  {rel} [IsTrans α rel]
-  {t₁ : PCotree? ι₁ α} {t₂ : PCotree? ι₂ α} {t₃ : PCotree? ι₃ α}
-  (h1 : PCotree?.Sim? rel t₁ t₂)
-  (h2 : PCotree?.Sim? rel t₂ t₃) : PCotree?.Sim? rel t₁ t₃ :=
-  Node.SimRel.trans h1 h2
+-- theorem PCotree?.Sim?.trans {ι₁ ι₂ ι₃ α} [BinderList α]
+--   {rel} [IsTrans α rel]
+--   {t₁ : PCotree? ι₁ α} {t₂ : PCotree? ι₂ α} {t₃ : PCotree? ι₃ α}
+--   (h1 : PCotree?.Sim? rel t₁ t₂)
+--   (h2 : PCotree?.Sim? rel t₂ t₃) : PCotree?.Sim? rel t₁ t₃ :=
+--   Node.SimRel.trans h1 h2
 
-theorem PCotree?.Sim?.lhs {ι₁ ι₂ α} [BinderList α]
-  {rel} [IsSymm α rel] [IsTrans α rel]
-  {t₁ : PCotree? ι₁ α} {t₂ : PCotree? ι₂ α}
-  (h : PCotree?.Sim? rel t₁ t₂) : PCotree?.Sim? rel t₁ t₁ :=
-  h.trans h.symm
+-- theorem PCotree?.Sim?.lhs {ι₁ ι₂ α} [BinderList α]
+--   {rel} [IsSymm α rel] [IsTrans α rel]
+--   {t₁ : PCotree? ι₁ α} {t₂ : PCotree? ι₂ α}
+--   (h : PCotree?.Sim? rel t₁ t₂) : PCotree?.Sim? rel t₁ t₁ :=
+--   h.trans h.symm
 
-theorem PCotree?.Sim?.rhs {ι₁ ι₂ α} [BinderList α]
-  {rel} [IsSymm α rel] [IsTrans α rel]
-  {t₁ : PCotree? ι₁ α} {t₂ : PCotree? ι₂ α}
-  (h : PCotree?.Sim? rel t₁ t₂) : PCotree?.Sim? rel t₂ t₂ :=
-  h.symm.lhs
+-- theorem PCotree?.Sim?.rhs {ι₁ ι₂ α} [BinderList α]
+--   {rel} [IsSymm α rel] [IsTrans α rel]
+--   {t₁ : PCotree? ι₁ α} {t₂ : PCotree? ι₂ α}
+--   (h : PCotree?.Sim? rel t₁ t₂) : PCotree?.Sim? rel t₂ t₂ :=
+--   h.symm.lhs
 
-def PCotree?.Undef {ι α} [BinderList α]
-  (rel : α → α → Prop)
-  (t : PCotree? ι α) : Prop
-  := ¬ PCotree?.Sim? rel t t
+-- def PCotree?.Undef {ι α} [BinderList α]
+--   (rel : α → α → Prop)
+--   (t : PCotree? ι α) : Prop
+--   := ¬ PCotree?.Sim? rel t t
 
-theorem PCotree?.Undef.not_lhs {ι₁ ι₂ α} [BinderList α]
-  {rel : α → α → Prop} [IsSymm α rel] [IsTrans α rel]
-  {t₁ : PCotree? ι₁ α} {t₂ : PCotree? ι₂ α}
-  (h : PCotree?.Undef rel t₁) : ¬ PCotree?.Sim? rel t₁ t₂ :=
-  fun hsim => h hsim.lhs
+-- theorem PCotree?.Undef.not_lhs {ι₁ ι₂ α} [BinderList α]
+--   {rel : α → α → Prop} [IsSymm α rel] [IsTrans α rel]
+--   {t₁ : PCotree? ι₁ α} {t₂ : PCotree? ι₂ α}
+--   (h : PCotree?.Undef rel t₁) : ¬ PCotree?.Sim? rel t₁ t₂ :=
+--   fun hsim => h hsim.lhs
 
-theorem PCotree?.Undef.not_rhs {ι₁ ι₂ α} [BinderList α]
-  {rel : α → α → Prop} [IsSymm α rel] [IsTrans α rel]
-  {t₁ : PCotree? ι₁ α} {t₂ : PCotree? ι₂ α}
-  (h : PCotree?.Undef rel t₂) : ¬ PCotree?.Sim? rel t₁ t₂ :=
-  fun hsim => h hsim.rhs
+-- theorem PCotree?.Undef.not_rhs {ι₁ ι₂ α} [BinderList α]
+--   {rel : α → α → Prop} [IsSymm α rel] [IsTrans α rel]
+--   {t₁ : PCotree? ι₁ α} {t₂ : PCotree? ι₂ α}
+--   (h : PCotree?.Undef rel t₂) : ¬ PCotree?.Sim? rel t₁ t₂ :=
+--   fun hsim => h hsim.rhs
 
-def PCotree?.Sim {ι₁ ι₂ α} [BinderList α] (rel : α → α → Prop)
-  (t₁ : PCotree? ι₁ α) (t₂ : PCotree? ι₂ α) : Prop
-  := t₁.Sim? rel t₂ ∨ (t₁.Undef rel ∧ t₂.Undef rel)
+-- def PCotree?.Sim {ι₁ ι₂ α} [BinderList α] (rel : α → α → Prop)
+--   (t₁ : PCotree? ι₁ α) (t₂ : PCotree? ι₂ α) : Prop
+--   := t₁.Sim? rel t₂ ∨ (t₁.Undef rel ∧ t₂.Undef rel)
 
-theorem PCotree?.Sim.refl {ι α} [BinderList α]
-  {rel} [IsRefl α rel]
-  (t : PCotree? ι α) : PCotree?.Sim rel t t :=
-  open Classical in
-  if h : t.Sim? rel t then
-    Or.inl h
-  else
-    Or.inr ⟨h, h⟩
+-- theorem PCotree?.Sim.refl {ι α} [BinderList α]
+--   {rel} [IsRefl α rel]
+--   (t : PCotree? ι α) : PCotree?.Sim rel t t :=
+--   open Classical in
+--   if h : t.Sim? rel t then
+--     Or.inl h
+--   else
+--     Or.inr ⟨h, h⟩
 
-theorem PCotree?.Sim.symm {ι₁ ι₂ α} [BinderList α]
-  {rel} [IsSymm α rel]
-  {t₁ : PCotree? ι₁ α} {t₂ : PCotree? ι₂ α}
-  (h : PCotree?.Sim rel t₁ t₂) : PCotree?.Sim rel t₂ t₁ :=
-  match h with
-  | Or.inl hsim => Or.inl (PCotree?.Sim?.symm hsim)
-  | Or.inr ⟨h1, h2⟩ => Or.inr ⟨h2, h1⟩
+-- theorem PCotree?.Sim.symm {ι₁ ι₂ α} [BinderList α]
+--   {rel} [IsSymm α rel]
+--   {t₁ : PCotree? ι₁ α} {t₂ : PCotree? ι₂ α}
+--   (h : PCotree?.Sim rel t₁ t₂) : PCotree?.Sim rel t₂ t₁ :=
+--   match h with
+--   | Or.inl hsim => Or.inl (PCotree?.Sim?.symm hsim)
+--   | Or.inr ⟨h1, h2⟩ => Or.inr ⟨h2, h1⟩
 
-theorem PCotree?.Sim.trans {ι₁ ι₂ ι₃ α} [BinderList α]
-  {rel} [IsSymm α rel] [IsTrans α rel]
-  {t₁ : PCotree? ι₁ α} {t₂ : PCotree? ι₂ α} {t₃ : PCotree? ι₃ α}
-  (h1 : PCotree?.Sim rel t₁ t₂)
-  (h2 : PCotree?.Sim rel t₂ t₃) : PCotree?.Sim rel t₁ t₃ :=
-  match h1, h2 with
-  | Or.inl hsim1, Or.inl hsim2 => Or.inl (PCotree?.Sim?.trans hsim1 hsim2)
-  | Or.inl hsim1, Or.inr ⟨h2_undef1, _⟩ => (h2_undef1.not_rhs hsim1).elim
-  | Or.inr ⟨_, h1_undef2⟩, Or.inl hsim2 => (h1_undef2.not_lhs hsim2).elim
-  | Or.inr ⟨h1_undef1, _⟩, Or.inr ⟨_, h2_undef2⟩ =>
-    Or.inr ⟨h1_undef1, h2_undef2⟩
+-- theorem PCotree?.Sim.trans {ι₁ ι₂ ι₃ α} [BinderList α]
+--   {rel} [IsSymm α rel] [IsTrans α rel]
+--   {t₁ : PCotree? ι₁ α} {t₂ : PCotree? ι₂ α} {t₃ : PCotree? ι₃ α}
+--   (h1 : PCotree?.Sim rel t₁ t₂)
+--   (h2 : PCotree?.Sim rel t₂ t₃) : PCotree?.Sim rel t₁ t₃ :=
+--   match h1, h2 with
+--   | Or.inl hsim1, Or.inl hsim2 => Or.inl (PCotree?.Sim?.trans hsim1 hsim2)
+--   | Or.inl hsim1, Or.inr ⟨h2_undef1, _⟩ => (h2_undef1.not_rhs hsim1).elim
+--   | Or.inr ⟨_, h1_undef2⟩, Or.inl hsim2 => (h1_undef2.not_lhs hsim2).elim
+--   | Or.inr ⟨h1_undef1, _⟩, Or.inr ⟨_, h2_undef2⟩ =>
+--     Or.inr ⟨h1_undef1, h2_undef2⟩
 
-instance PCotree?.setoid (ι α) [BinderList α] : Setoid (PCotree? ι α) where
-  r := PCotree?.Sim Eq
-  iseqv := ⟨Sim.refl, Sim.symm, Sim.trans⟩
+-- instance PCotree?.setoid (ι α) [BinderList α] : Setoid (PCotree? ι α) where
+--   r := PCotree?.Sim Eq
+--   iseqv := ⟨Sim.refl, Sim.symm, Sim.trans⟩
 
-def Cotree? (ι : Type _) (α : Type _) [BinderList α] : Type _
-  := Quotient (PCotree?.setoid ι α)
+-- def Cotree? (ι : Type _) (α : Type _) [BinderList α] : Type _
+--   := Quotient (PCotree?.setoid ι α)
 
-instance PCotree?.instEmptyCollection {ι α} [Inhabited ι] [BinderList α]
-  : EmptyCollection (PCotree? ι α) where
-  emptyCollection := {
-    ix := default,
-    getNode := fun _ => none
-  }
+-- instance PCotree?.instEmptyCollection {ι α} [Inhabited ι] [BinderList α]
+--   : EmptyCollection (PCotree? ι α) where
+--   emptyCollection := {
+--     ix := default,
+--     getNode := fun _ => none
+--   }
 
-instance PCotree?.instInhabited {ι α} [Inhabited ι] [BinderList α]
-  : Inhabited (PCotree? ι α) := ⟨∅⟩
+-- instance PCotree?.instInhabited {ι α} [Inhabited ι] [BinderList α]
+--   : Inhabited (PCotree? ι α) := ⟨∅⟩
 
-def PCotree?.toCotree? {ι α} [BinderList α] (t : PCotree? ι α) : Cotree? ι α := ⟦t⟧
+-- def PCotree?.toCotree? {ι α} [BinderList α] (t : PCotree? ι α) : Cotree? ι α := ⟦t⟧
 
-instance Cotree?.instEmptyCollection {ι α} [Inhabited ι] [BinderList α]
-  : EmptyCollection (Cotree? ι α) where
-  emptyCollection := PCotree?.toCotree? (∅ : PCotree? ι α)
+-- instance Cotree?.instEmptyCollection {ι α} [Inhabited ι] [BinderList α]
+--   : EmptyCollection (Cotree? ι α) where
+--   emptyCollection := PCotree?.toCotree? (∅ : PCotree? ι α)
 
-instance Cotree?.instInhabited {ι α} [Inhabited ι] [BinderList α]
-  : Inhabited (Cotree? ι α) := ⟨∅⟩
+-- instance Cotree?.instInhabited {ι α} [Inhabited ι] [BinderList α]
+--   : Inhabited (Cotree? ι α) := ⟨∅⟩
 
 /-- A pre-cotree over a finite address space -/
 structure PFCotree (α : Type _) [NumChildren α] where
@@ -783,68 +782,68 @@ structure PFCotree? (α : Type _) [NumChildren α] where
   size : ℕ
   cotree : PCotree? (Fin size) α
 
-def PFCotree?.Sim? {α β} [BinderList α] [BinderList β] (rel : α → β → Prop)
-  (t₁ : PFCotree? α) (t₂ : PFCotree? β) : Prop
-  := t₁.cotree.Sim? rel t₂.cotree
+-- def PFCotree?.Sim? {α β} [BinderList α] [BinderList β] (rel : α → β → Prop)
+--   (t₁ : PFCotree? α) (t₂ : PFCotree? β) : Prop
+--   := t₁.cotree.Sim? rel t₂.cotree
 
-theorem PFCotree?.Sim?.symm {α} [BinderList α]
-  {rel} [IsSymm α rel]
-  {t₁ : PFCotree? α} {t₂ : PFCotree? α}
-  (h : PFCotree?.Sim? rel t₁ t₂) : PFCotree?.Sim? rel t₂ t₁ :=
-  PCotree?.Sim?.symm h
+-- theorem PFCotree?.Sim?.symm {α} [BinderList α]
+--   {rel} [IsSymm α rel]
+--   {t₁ : PFCotree? α} {t₂ : PFCotree? α}
+--   (h : PFCotree?.Sim? rel t₁ t₂) : PFCotree?.Sim? rel t₂ t₁ :=
+--   PCotree?.Sim?.symm h
 
-theorem PFCotree?.Sim?.trans {α} [BinderList α]
-  {rel} [IsTrans α rel]
-  {t₁ : PFCotree? α} {t₂ : PFCotree? α} {t₃ : PFCotree? α}
-  (h1 : PFCotree?.Sim? rel t₁ t₂)
-  (h2 : PFCotree?.Sim? rel t₂ t₃) : PFCotree?.Sim? rel t₁ t₃ :=
-  PCotree?.Sim?.trans h1 h2
+-- theorem PFCotree?.Sim?.trans {α} [BinderList α]
+--   {rel} [IsTrans α rel]
+--   {t₁ : PFCotree? α} {t₂ : PFCotree? α} {t₃ : PFCotree? α}
+--   (h1 : PFCotree?.Sim? rel t₁ t₂)
+--   (h2 : PFCotree?.Sim? rel t₂ t₃) : PFCotree?.Sim? rel t₁ t₃ :=
+--   PCotree?.Sim?.trans h1 h2
 
-def PFCotree?.Sim {α} [BinderList α] (rel : α → α → Prop)
-  (t₁ : PFCotree? α) (t₂ : PFCotree? α) : Prop
-  := t₁.cotree.Sim rel t₂.cotree
+-- def PFCotree?.Sim {α} [BinderList α] (rel : α → α → Prop)
+--   (t₁ : PFCotree? α) (t₂ : PFCotree? α) : Prop
+--   := t₁.cotree.Sim rel t₂.cotree
 
-theorem PFCotree?.Sim.refl {α} [BinderList α]
-  {rel} [IsRefl α rel]
-  (t : PFCotree? α) : PFCotree?.Sim rel t t :=
-  PCotree?.Sim.refl t.cotree
+-- theorem PFCotree?.Sim.refl {α} [BinderList α]
+--   {rel} [IsRefl α rel]
+--   (t : PFCotree? α) : PFCotree?.Sim rel t t :=
+--   PCotree?.Sim.refl t.cotree
 
-theorem PFCotree?.Sim.symm {α} [BinderList α]
-  {rel} [IsSymm α rel]
-  {t₁ : PFCotree? α} {t₂ : PFCotree? α}
-  (h : PFCotree?.Sim rel t₁ t₂) : PFCotree?.Sim rel t₂ t₁ :=
-  PCotree?.Sim.symm h
+-- theorem PFCotree?.Sim.symm {α} [BinderList α]
+--   {rel} [IsSymm α rel]
+--   {t₁ : PFCotree? α} {t₂ : PFCotree? α}
+--   (h : PFCotree?.Sim rel t₁ t₂) : PFCotree?.Sim rel t₂ t₁ :=
+--   PCotree?.Sim.symm h
 
-theorem PFCotree?.Sim.trans {α} [BinderList α]
-  {rel} [IsSymm α rel] [IsTrans α rel]
-  {t₁ : PFCotree? α} {t₂ : PFCotree? α} {t₃ : PFCotree? α}
-  (h1 : PFCotree?.Sim rel t₁ t₂)
-  (h2 : PFCotree?.Sim rel t₂ t₃) : PFCotree?.Sim rel t₁ t₃ :=
-  PCotree?.Sim.trans h1 h2
+-- theorem PFCotree?.Sim.trans {α} [BinderList α]
+--   {rel} [IsSymm α rel] [IsTrans α rel]
+--   {t₁ : PFCotree? α} {t₂ : PFCotree? α} {t₃ : PFCotree? α}
+--   (h1 : PFCotree?.Sim rel t₁ t₂)
+--   (h2 : PFCotree?.Sim rel t₂ t₃) : PFCotree?.Sim rel t₁ t₃ :=
+--   PCotree?.Sim.trans h1 h2
 
-instance PFCotree?.setoid (α) [BinderList α] : Setoid (PFCotree? α) where
-  r := PFCotree?.Sim Eq
-  iseqv := ⟨Sim.refl, Sim.symm, Sim.trans⟩
+-- instance PFCotree?.setoid (α) [BinderList α] : Setoid (PFCotree? α) where
+--   r := PFCotree?.Sim Eq
+--   iseqv := ⟨Sim.refl, Sim.symm, Sim.trans⟩
 
-def FCotree? (α : Type _) [BinderList α] : Type _ := Quotient (PFCotree?.setoid α)
+-- def FCotree? (α : Type _) [BinderList α] : Type _ := Quotient (PFCotree?.setoid α)
 
-def PFCotree?.toFCotree? {α} [BinderList α] (t : PFCotree? α) : FCotree? α := ⟦t⟧
+-- def PFCotree?.toFCotree? {α} [BinderList α] (t : PFCotree? α) : FCotree? α := ⟦t⟧
 
-instance PFCotree?.instEmptyCollection {α} [Inhabited α] [BinderList α]
-  : EmptyCollection (PFCotree? α) where
-  emptyCollection := {
-    size := 1,
-    cotree := ∅
-  }
+-- instance PFCotree?.instEmptyCollection {α} [Inhabited α] [BinderList α]
+--   : EmptyCollection (PFCotree? α) where
+--   emptyCollection := {
+--     size := 1,
+--     cotree := ∅
+--   }
 
-instance PFCotree?.instInhabited {α} [Inhabited α] [BinderList α]
-  : Inhabited (PFCotree? α) := ⟨∅⟩
+-- instance PFCotree?.instInhabited {α} [Inhabited α] [BinderList α]
+--   : Inhabited (PFCotree? α) := ⟨∅⟩
 
-instance FCotree?.instEmptyCollection {α} [Inhabited α] [BinderList α]
-  : EmptyCollection (FCotree? α) where
-  emptyCollection := PFCotree?.toFCotree? (∅ : PFCotree? α)
+-- instance FCotree?.instEmptyCollection {α} [Inhabited α] [BinderList α]
+--   : EmptyCollection (FCotree? α) where
+--   emptyCollection := PFCotree?.toFCotree? (∅ : PFCotree? α)
 
-instance FCotree?.instInhabited {α} [Inhabited α] [BinderList α]
-  : Inhabited (FCotree? α) := ⟨∅⟩
+-- instance FCotree?.instInhabited {α} [Inhabited α] [BinderList α]
+--   : Inhabited (FCotree? α) := ⟨∅⟩
 
 end Gt3
